src/program_proof/lockservice/kv_proof.v
@@ -30,37 +30,64 @@ Definition Get_Post γ va : RPCValsC -> u64 -> iProp Σ := λ args v, (⌜v = va
 Definition Put_Pre γ : RPCValsC -> iProp Σ := (λ args, args.(U64_1) [[γ.(ks_kvMapGN)]]↦ _)%I.
 Definition Put_Post γ : RPCValsC -> u64 -> iProp Σ := (λ args _, args.(U64_1) [[γ.(ks_kvMapGN)]]↦ args.(U64_2))%I.
 
-Definition KVServer_own_core γ (srv:loc) : iProp Σ :=
-  ∃ (kvs_ptr:loc) (kvsM:gmap u64 u64),
-  "HlocksOwn" ∷ srv ↦[KVServer.S :: "kvs"] #kvs_ptr
-∗ "HkvsMap" ∷ is_map (kvs_ptr) kvsM
-∗ "Hkvctx" ∷ map_ctx γ.(ks_kvMapGN) 1 kvsM
-.
-
 (* FIXME: this is currently just a placeholder *)
-Definition own_kvclerk γ ck_ptr (srv : u64) : iProp Σ :=
+Definition KVClerk_own γ ck_ptr (host : string) : iProp Σ :=
   ∃ (cl_ptr:loc),
    "Hcl_ptr" ∷ ck_ptr ↦[KVClerk.S :: "client"] #cl_ptr ∗
-   "Hprimary" ∷ ck_ptr ↦[KVClerk.S :: "primary"] #srv ∗
-   "Hcl" ∷ own_rpcclient cl_ptr γ.(ks_rpcGN).
+   "Hprimary" ∷ ck_ptr ↦[KVClerk.S :: "primary"] #(str host) ∗
+   "Hcl" ∷ RPCClient_own cl_ptr host γ.(ks_rpcGN).
 
-Definition is_kvserver γ (srv:loc) : iProp Σ :=
-  ∃ (sv:loc),
-  "#Hsv" ∷ readonly (srv ↦[KVServer.S :: "sv"] #sv) ∗
-  "#His_rpc" ∷ is_rpcserver sv γ.(ks_rpcGN) (KVServer_own_core γ srv)
+Print is_lock.
+
+Definition KVServer_own_core γ srv kvsM : iProp Σ :=
+  ∃ (kvs_ptr:loc),
+  "HlocksOwn" ∷ srv ↦[KVServer.S :: "kvs"] #kvs_ptr ∗
+  "HkvsMap" ∷ is_map (kvs_ptr) kvsM ∗
+  "Hkvctx" ∷ map_ctx γ.(ks_kvMapGN) 1 kvsM (* ghost part *)
 .
 
-Lemma put_core_spec γ (srv:loc) args :
-{{{ 
-     KVServer_own_core γ srv ∗ Put_Pre γ args
-}}}
-  KVServer__put_core #srv (into_val.to_val args)
+Definition KVServer_mutex_inv γ (srv:loc) : iProp Σ :=
+  ∃ (sv:loc) (kvsM lastSeqM lastReplyM:gmap u64 u64),
+  "Hcore" ∷ KVServer_own_core γ srv kvsM ∗
+  "Hsv" ∷ srv ↦[KVServer.S :: "sv"] #sv ∗
+  "Hrpc_vol" ∷ RPCServer_own_vol sv γ.(ks_rpcGN) lastSeqM lastReplyM ∗
+  "Hrpc_ghost" ∷ RPCServer_own_ghost γ.(ks_rpcGN) lastSeqM lastReplyM
+.
+
+Definition mutexN := nroot .@ "kvservermutex".
+
+Definition is_kvserver γ (srv:loc) : iProp Σ :=
+  ∃ mu,
+  "#Hmu" ∷ readonly (srv ↦[KVServer.S :: "mu"] mu) ∗
+  "#His_rpc" ∷ is_lock mutexN mu (KVServer_mutex_inv γ srv)
+.
+
+Lemma put_core_spec γ (srv:loc) :
 {{{
-   RET #0; KVServer_own_core γ srv
-      ∗ Put_Post γ args 0
+     True
+}}}
+  KVServer__put_core #srv
+{{{
+     (f:goose_lang.val), RET f;
+     ∀ args kvsM,
+     {{{
+         KVServer_own_core γ srv kvsM ∗ ▷ Put_Pre γ args
+     }}}
+        f (into_val.to_val args)
+      {{{
+           kvsM', RET #0; KVServer_own_core γ srv kvsM'
+                                            ∗ ▷ Put_Post γ args 0
+      }}}
 }}}.
 Proof.
-  iIntros (Φ) "[Hksown Hpre] Hpost".
+  iIntros (Φ) "_ HΦ".
+  wp_lam.
+  wp_pures.
+  iApply "HΦ".
+  iIntros (??).
+  clear Φ.
+
+  iIntros (Φ) "!# [Hksown Hpre] Hpost".
   wp_lam.
   wp_pures.
   iNamed "Hksown".
@@ -71,20 +98,35 @@ Proof.
   iMod (map_update with "Hkvctx Hpre") as "[Hkvctx Hptsto]".
   wp_seq.
   iApply "Hpost".
-  iFrame. iExists _, _; iFrame.
+  iFrame. iExists _; iFrame.
 Qed.
 
-Lemma get_core_spec (srv:loc) args (va:u64) γ :
-{{{ 
-     KVServer_own_core γ srv ∗ Get_Pre γ va args
-}}}
-  KVServer__get_core #srv (into_val.to_val args)%V
+Lemma get_core_spec (srv:loc) γ :
 {{{
-   r, RET #r; KVServer_own_core γ srv ∗
-   Get_Post γ va args r
+     True
+}}}
+  KVServer__get_core #srv
+{{{
+     (f:goose_lang.val), RET f;
+     ∀ args va kvsM,
+     {{{
+         KVServer_own_core γ srv kvsM ∗ ▷ Get_Pre γ va args
+     }}}
+        f (into_val.to_val args)
+      {{{
+           kvsM', RET #va; KVServer_own_core γ srv kvsM'
+                                            ∗ ▷ Get_Post γ va args va
+      }}}
 }}}.
 Proof.
-  iIntros (Φ) "[Hksown Hpre] Hpost".
+  iIntros (Φ) "_ HΦ".
+  wp_lam.
+  wp_pures.
+  iApply "HΦ".
+  iIntros (???).
+  clear Φ.
+
+  iIntros (Φ) "!# [Hksown Hpre] Hpost".
   wp_lam.
   wp_pures.
   iNamed "Hksown".
@@ -106,7 +148,7 @@ Proof.
   wp_pures.
   iApply "Hpost".
   iFrame.
-  iSplit; last done. iExists _, _; iFrame.
+  iSplit; last done. iExists _; iFrame.
 Qed.
 
 Lemma KVServer__Get_spec srv γ :
@@ -116,7 +158,7 @@ is_kvserver γ srv -∗
 }}}
     KVServer__Get #srv
 {{{ (f:goose_lang.val), RET f;
-        ∀ args req va, is_rpcHandler f γ.(ks_rpcGN) args req (Get_Pre γ va args) (Get_Post γ va args)
+        ∀ va, is_rpcHandlerEncoded f γ.(ks_rpcGN) (Get_Pre γ va) (Get_Post γ va)
 }}}.
 Proof.
   iIntros "#Hls".
@@ -124,17 +166,61 @@ Proof.
   wp_lam.
   wp_pures.
   iApply "Hpost".
-  iIntros (args req).
-  iIntros (????).
-  iIntros (_ _).
-  iNamed "Hls". wp_pures.
-  wp_loadField.
-  iApply (RPCServer__HandleRequest_spec with "[] His_rpc"); last by eauto.
-  clear Φ. iIntros "!#" (Φ) "Hpre HΦ".
+  iIntros (?).
+  clear Φ.
+  iIntros (?????? Φ) "!# Hpre HΦ".
+  iNamed "Hpre".
   wp_pures.
-  iApply (get_core_spec with "Hpre"); last by eauto.
+  iNamed "Hls".
+  wp_loadField.
+  wp_apply (acquire_spec with "[$His_rpc]").
+  iIntros "[Hlocked Hown]".
+  iNamed "Hown".
+  wp_pures.
+  wp_apply (get_core_spec srv γ).
+  iIntros (fget) "#Hfget".
+  wp_pures.
+  wp_loadField.
+  wp_apply (RPCServer__HandleRequest_spec _ _ _ _ (KVServer_own_core γ srv kvsM) (∃ kvsM', KVServer_own_core γ srv kvsM')%I _ _ _ with "[] [Hargs Hrpc_vol Hrpc_ghost Hreply Hcore]").
+  {
+    clear Φ.
+    iIntros (Φ) "!# Hpre HΦ".
+    wp_apply ("Hfget" with "[- HΦ]").
+    {
+      iDestruct "Hpre" as "[$ Hpre]".
+      iFrame "Hpre".
+    }
+    iIntros (?) "[Hctx' Hpost]".
+    iApply "HΦ".
+    iFrame.
+    iExists _; iFrame.
+  }
+  {
+    iFrame "∗ #".
+    iExists _; iFrame.
+  }
+  iIntros (?) "HH".
+  iDestruct "HH" as (??) "(Hrpc_vol & Hrpc_ghost & Hreply & #Hpost & Hkv_own)".
+  wp_pures.
+  wp_loadField.
+  wp_apply (release_spec with "[$His_rpc $Hlocked Hrpc_vol Hrpc_ghost Hkv_own Hsv]").
+  {
+    iNext.
+    iDestruct "Hkv_own" as "[Hkv_own|Hkv_own]".
+    { iExists _, _, _, _. iFrame. }
+    {
+      iDestruct "Hkv_own" as (?) "H".
+      iExists _, _, _, _. iFrame.
+    }
+  }
+
+  wp_pures.
+  iApply "HΦ".
+  iExists _; iFrame.
+  iFrame "Hpost".
 Qed.
 
+(*
 Lemma KVServer__Put_spec srv γ :
 is_kvserver γ srv -∗
 {{{
@@ -160,27 +246,25 @@ Proof.
   wp_pures.
   iApply (put_core_spec with "Hpre"); last by eauto.
 Qed.
+*)
+
 (* TODO: see if any more repetition can be removed *)
 
-Definition is_kvserver_host γ (host:u64) : iProp Σ :=
-  ∃ handlers (fget fput : val),
-    "#Hhost" ∷ host [[rpcreg_gname]]↦ro handlers ∗
-    "%Hhandler_get" ∷ ⌜handlers !! (U64 2) = Some fget⌝ ∗
-    "%Hhandler_put" ∷ ⌜handlers !! (U64 1) = Some fput⌝ ∗
-    "#Hgetspec" ∷ (∀ args req va,
-      is_rpcHandlerHost host (U64 2) γ.(ks_rpcGN) args req (Get_Pre γ va args) (Get_Post γ va args)) ∗
-    "#Hputspec" ∷ (∀ args req,
-      is_rpcHandlerHost host (U64 1) γ.(ks_rpcGN) args req (Put_Pre γ args) (Put_Post γ args)) ∗
-    "#Hisrpcserver" ∷ is_RPCServer γ.(ks_rpcGN).
+Definition is_kvserver_host γ (host:string) : iProp Σ :=
+    "#Hputspec" ∷ (
+      handler_is2 host (U64 1) γ.(ks_rpcGN) (Put_Pre γ) (Put_Post γ)) ∗
+    "#Hgetspec" ∷ (∀ va,
+      handler_is2 host (U64 2) γ.(ks_rpcGN) (Get_Pre γ va) (Get_Post γ va)) ∗
+    "#Hrpcserver" ∷ is_RPCServer γ.(ks_rpcGN).
 
-Lemma KVClerk__Get_spec (kck:loc) (srv:u64) (key va:u64) γ  :
+Lemma KVClerk__Get_spec (kck:loc) (srv:string) (key va:u64) γ  :
 is_kvserver_host γ srv -∗
 {{{
-     own_kvclerk γ kck srv ∗ (key [[γ.(ks_kvMapGN)]]↦ va)
+     KVClerk_own γ kck srv ∗ (key [[γ.(ks_kvMapGN)]]↦ va)
 }}}
   KVClerk__Get #kck #key
 {{{
-     v, RET #v; ⌜v = va⌝ ∗ own_kvclerk γ kck srv ∗ (key [[γ.(ks_kvMapGN)]]↦ va )
+     v, RET #v; ⌜v = va⌝ ∗ KVClerk_own γ kck srv ∗ (key [[γ.(ks_kvMapGN)]]↦ va )
 }}}.
 Proof.
   iIntros "#Hserver" (Φ) "!# (Hclerk & Hpre) Hpost".
@@ -190,7 +274,6 @@ Proof.
   repeat wp_loadField.
   wp_apply (RPCClient__MakeRequest_spec _ _ _ {|U64_1:=_ ; U64_2:= _ |} γ.(ks_rpcGN) with "[] [Hpre Hcl]"); eauto.
   {
-    iIntros (req).
     iNamed "Hserver".
     iApply "Hgetspec".
   }
@@ -206,15 +289,15 @@ Proof.
   iExists _; iFrame.
 Qed.
 
-Lemma KVClerk__Put_spec (kck:loc) (srv:u64) (key va:u64) γ :
+Lemma KVClerk__Put_spec (kck:loc) (srv:string) (key va:u64) γ :
 is_kvserver_host γ srv -∗
 {{{
-     own_kvclerk γ kck srv ∗ (key [[γ.(ks_kvMapGN)]]↦ _ )
+     KVClerk_own γ kck srv ∗ (key [[γ.(ks_kvMapGN)]]↦ _ )
 }}}
   KVClerk__Put #kck #key #va
 {{{
      RET #();
-     own_kvclerk γ kck srv ∗ (key [[γ.(ks_kvMapGN)]]↦ va )
+     KVClerk_own γ kck srv ∗ (key [[γ.(ks_kvMapGN)]]↦ va )
 }}}.
 Proof.
   iIntros "#Hserver" (Φ) "!# (Hclerk & Hpre) Hpost".
@@ -224,7 +307,6 @@ Proof.
   repeat wp_loadField.
   wp_apply (RPCClient__MakeRequest_spec _ _ _ {| U64_1:= _; U64_2:=_ |} γ.(ks_rpcGN) with "[] [Hpre Hcl]"); eauto.
   {
-    iIntros (req).
     iNamed "Hserver". iApply "Hputspec".
   }
   {
@@ -239,7 +321,7 @@ Proof.
 Qed.
 
 Definition kvserver_cid_token γ cid :=
-  RPCClient_own γ.(ks_rpcGN) cid 1.
+  RPCClient_own_ghost γ.(ks_rpcGN) cid 1.
 
 Lemma MakeKVServer_spec :
   {{{ True }}}
@@ -256,41 +338,60 @@ Proof.
 
   wp_apply wp_allocStruct; first by eauto.
   iIntros (l) "Hl". wp_pures.
-  iDestruct (struct_fields_split with "Hl") as "(l_sv & l_locks & _)".
+  iDestruct (struct_fields_split with "Hl") as "(l_mu & l_sv & l_kvs & _)".
+  wp_apply (wp_new_free_lock).
+  iIntros (mu) "Hmu".
+  wp_storeField.
   wp_apply (wp_NewMap u64 (t:=uint64T)). iIntros (kvs) "Hkvs".
   wp_storeField.
-  wp_apply (MakeRPCServer_spec (KVServer_own_core γ l) with "[$server_own $is_server l_locks Hγkv Hkvs]").
-  { iExists _, _. iFrame. }
-  iIntros (sv) "#Hsv".
+  wp_apply (MakeRPCServer_spec with "[$is_server]").
+  iIntros (sv) "Hrpcown".
   wp_storeField.
   iApply ("HΦ" $! γ).
   iFrame "cli_tokens".
-  iExists sv. iFrame "#".
-  by iMod (readonly_alloc_1 with "l_sv") as "$".
+  iExists _.
+  iMod (readonly_alloc_1 with "l_mu") as "$".
+  iApply (alloc_lock with "Hmu [-]").
+  iExists _, _, _, _.
+  iNext.
+  iFrame "∗#".
+  iExists _.
+  iFrame.
 Qed.
 (* TODO: return all of the ptsto's here; update KVServer_own_core so it has map_ctx bigger than the physical map *)
 
 Opaque zero_val.
 Lemma KVServer_AllocServer_spec γ srv :
-  {{{ is_kvserver γ srv }}}
-    KVServer__AllocServer #srv
-  {{{ (host:u64), RET #host;
-    is_kvserver_host γ host
-  }}}.
+is_kvserver γ srv -∗
+  {{{ True }}}
+    KVServer__Start #srv
+  {{{ RET #(); True }}}.
 Proof.
-  iIntros (Φ) "#Hsrv HΦ".
+  iIntros "#Hsrv !#" (Φ) "_ HΦ".
   wp_lam.
   wp_apply map.wp_NewMap.
   iIntros (mref) "Hm".
   wp_pures.
-  wp_apply KVServer__Put_spec; first eauto.
-  iIntros (fput) "#Hfput".
-  wp_apply (map.wp_MapInsert with "Hm").
+  wp_lam.
+  wp_apply (wp_ConjugateRpcFunc with "[]").
+  {
+    admit.
+  }
+  iIntros (fput) "#Hputspec".
+
+  wp_apply (map.wp_MapInsert with "[$Hm]").
   iIntros "Hm".
+  unfold map.map_insert.
+  rewrite insert_empty.
+
   wp_pures.
-  wp_apply KVServer__Get_spec; first eauto.
+  wp_apply (KVServer__Get_spec with "Hsrv").
   iIntros (fget) "#Hfget".
-  wp_apply (map.wp_MapInsert with "Hm").
+  wp_apply (wp_ConjugateRpcFunc with "[]").
+  {
+    iApply "Hfget".
+  }
+
   iIntros "Hm".
   wp_apply (wp_AllocServer with "Hm").
   iIntros (host) "#Hhost".
@@ -327,10 +428,10 @@ Qed.
 Lemma MakeKVClerk_spec γ (srv : u64) (cid : u64) :
   {{{ is_kvserver_host γ srv ∗ kvserver_cid_token γ cid }}}
     MakeKVClerk #srv #cid
-  {{{ ck, RET #ck; own_kvclerk γ ck srv }}}.
+  {{{ ck, RET #ck; KVClerk_own γ ck srv }}}.
 Proof.
   iIntros (Φ) "[#Hserver Hcid] HΦ". wp_lam.
-  rewrite /kvserver_cid_token /own_kvclerk.
+  rewrite /kvserver_cid_token /KVClerk_own.
   iApply wp_fupd.
 
   wp_apply wp_allocStruct; first by eauto.
